\documentclass{article}
\usepackage{amsmath,amsthm,amssymb}

\newtheorem{theorem}{Theorem}
\newtheorem{lemma}{Lemma}
\newtheorem{definition}{Definition}

\begin{document}

\title{Sample Mathematical Content}
\author{Autoformalize Demo}
\date{\today}
\maketitle

\begin{definition}[Even Number]
\label{def:even}
A natural number $n$ is called even if there exists a natural number $k$ such that $n = 2k$.
\end{definition}

\begin{theorem}[Sum of Even Numbers]
\label{thm:sum_even}
The sum of two even numbers is even.
\end{theorem}

\begin{proof}
Let $a$ and $b$ be two even numbers. By the definition of even numbers, there exist natural numbers $k$ and $l$ such that $a = 2k$ and $b = 2l$.

Therefore, $a + b = 2k + 2l = 2(k + l)$.

Since $k + l$ is a natural number, we have shown that $a + b$ is even.
\end{proof}

\begin{lemma}[Zero is Even]
\label{lem:zero_even}
The number $0$ is even.
\end{lemma}

\begin{proof}
We can write $0 = 2 \cdot 0$, so by definition, $0$ is even.
\end{proof}

\begin{theorem}[Product Property]
If $n$ is even, then $n^2$ is even.
\end{theorem}

\begin{proof}
Let $n$ be even. Then there exists a natural number $k$ such that $n = 2k$.

Therefore, $n^2 = (2k)^2 = 4k^2 = 2(2k^2)$.

Since $2k^2$ is a natural number, we have shown that $n^2$ is even.
\end{proof}

\end{document}